# baseURI: http://linked.data.gov.au/def/loci
# imports: http://purl.org/linked-data/registry#
# imports: http://www.w3.org/ns/dcat#

@prefix : <http://linked.data.gov.au/def/loci#> .
@prefix dcat: <http://www.w3.org/ns/dcat#> .
@prefix dct: <http://purl.org/dc/terms/> .
@prefix doap: <http://usefulinc.com/ns/doap#> .
@prefix foaf: <http://xmlns.com/foaf/0.1/> .
@prefix geo: <http://www.opengis.net/ont/geosparql#> .
@prefix org: <http://www.w3.org/ns/org#> .
@prefix owl: <http://www.w3.org/2002/07/owl#> .
@prefix prof: <http://www.w3.org/ns/dx/prof/> .
@prefix prov: <http://www.w3.org/ns/prov#> .
@prefix rdf: <http://www.w3.org/1999/02/22-rdf-syntax-ns#> .
@prefix rdfs: <http://www.w3.org/2000/01/rdf-schema#> .
@prefix reg: <http://purl.org/linked-data/registry#> .
@prefix role: <http://www.w3.org/ns/dx/prof/role/> .
@prefix sdo: <https://schema.org/> .
@prefix skos: <http://www.w3.org/2004/02/skos/core#> .
@prefix void: <http://rdfs.org/ns/void#> .
@prefix xsd: <http://www.w3.org/2001/XMLSchema#> .

<http://catalogue.linked.data.gov.au/org/abs>
  a owl:NamedIndividual ;
  a org:Organization ;
  rdfs:label "Australian Bureau of Statistics" ;
.
<http://catalogue.linked.data.gov.au/org/csiro>
  a owl:NamedIndividual ;
  a org:Organization ;
  rdfs:label "CSIRO" ;
.
<http://catalogue.linked.data.gov.au/org/ga>
  a owl:NamedIndividual ;
  a org:Organization ;
  rdfs:label "Geoscience Australia" ;
.
<http://catalogue.linked.data.gov.au/org/psma>
  a owl:NamedIndividual ;
  a org:Organization ;
  rdfs:label "PSMA Australia" ;
.
<http://linked.data.gov.au/dataset/addrcatch>
  a :Linkset ;
  a owl:NamedIndividual ;
  rdfs:label "Addresses Catchments Linkset" ;
.
<http://linked.data.gov.au/dataset/asgs2016>
  a :Dataset ;
  a owl:NamedIndividual ;
  rdfs:label "ASGS 2016 Dataset" ;
.
<http://linked.data.gov.au/dataset/geofabric>
  a :Dataset ;
  a owl:NamedIndividual ;
  rdfs:label "Geofabric Dataset" ;
.
<http://linked.data.gov.au/dataset/gnaf>
  a :Dataset ;
  a owl:NamedIndividual ;
  rdfs:label "GNAF Dataset" ;
.
<http://linked.data.gov.au/dataset/gnaf-2016-05>
  a :Dataset ;
  a owl:NamedIndividual ;
  rdfs:label "GNAF 2016 May Dataset" ;
.
<http://linked.data.gov.au/def/loci>
  a owl:Ontology ;
  a prof:Profile ;
  dct:created "2018-10-29"^^xsd:date ;
  dct:creator [
      sdo:identifier <http://orcid.org/0000-0002-8742-7730> ;
      sdo:name "Nicholas J. Car" ;
    ] ;
  dct:modified "2019-06-04"^^xsd:date ;
  dct:publisher [
      sdo:identifier <http://catalogue.linked.data.gov.au/org/csiro> ;
      sdo:name "CSIRO" ;
    ] ;
  rdfs:comment """A profile of several ontologies implemented to govern Linked Data resources published within the LOC-I project.

This is a profile of the [GeoSPARQL](http://www.opengeospatial.org/standards/geosparql) and [DCAT v2](https://www.w3.org/TR/vocab-dcat-2/) & [VOID](http://www.w3.org/TR/void/) that require certain properties defined by those ontologies be present for several classes of resource that are of particular importance to the [LOC-I](https://confluence.csiro.au/display/DIPAAnalyticHubs/Location+Integration+Capability+Loc-I) project.

This ontology constrains both normative instruction on what constitutes LOC-I objects and supplies executable constraints to validate instances.""" ;
  rdfs:label "LOC-I Ontology"@en ;
  rdfs:label "LocI Ontology" ;
  rdfs:seeAlso "http://github.com/CSIRO-enviro-informatics/loci-ont/"@en ;
  owl:imports reg: ;
  owl:imports dcat: ;
  owl:versionIRI <http://linked.data.gov.au/def/loci/1.0> ;
  owl:versionInfo "Beta version"@en ;
  prof:hasResource [
      a prof:ResourceDescriptor ;
      dct:format <https://w3id.org/mediatype/image/svg> ;
      dct:title "Ontology overview image"@en ;
      prof:hasArtifact <http://linked.data.gov.au/def/loci/images/model.svg> ;
      prof:hasRole role:guidance ;
    ] ;
  prof:hasResource [
      a prof:ResourceDescriptor ;
      dct:format <https://w3id.org/mediatype/text/html> ;
      dct:title "Guidance document"@en ;
      prof:hasArtifact <http://linked.data.gov.au/def/loci/model.html> ;
      prof:hasRole role:guidance ;
    ] ;
  prof:hasResource [
      a prof:ResourceDescriptor ;
      dct:format <https://w3id.org/mediatype/text/turtle> ;
      dct:title "Profile Specification"@en ;
      prof:hasArtifact <http://linked.data.gov.au/def/loci/model.ttl> ;
      prof:hasRole role:specification ;
    ] ;
  prof:hasResource [
      a prof:ResourceDescriptor ;
      dct:format <https://w3id.org/mediatype/text/turtle> ;
      dct:title "Validator Shapes graph"@en ;
      prof:hasArtifact <http://linked.data.gov.au/def/loci/constraints.ttl> ;
      prof:hasRole role:constraints ;
    ] ;
  prof:isProfileOf reg: ;
  prof:isProfileOf void: ;
  prof:isProfileOf geo: ;
  prof:isProfileOf dcat: ;
  prof:isProfileOf org: ;
  prof:token "loci"^^xsd:token ;
  prov:wasGeneratedBy [
      a doap:Project ;
      a prov:Activity ;
      doap:repository <https://github.com/CSIRO-enviro-informatics/loci-ont> ;
      rdfs:label "Loc-I project" ;
    ] ;
.
:DataPublisher
  a owl:Class ;
  a owl:NamedIndividual ;
  rdfs:comment "The set of all approved publishers of LocI data, all of whom are known"@en ;
  rdfs:label "LocI Data Publishers" ;
  rdfs:subClassOf foaf:Group ;
  owl:equivalentClass [
      a owl:Class ;
      owl:oneOf (
          <http://catalogue.linked.data.gov.au/org/abs>
          <http://catalogue.linked.data.gov.au/org/csiro>
          <http://catalogue.linked.data.gov.au/org/ga>
          <http://catalogue.linked.data.gov.au/org/psma>
        ) ;
    ] ;
.
:Dataset
  a owl:Class ;
  rdfs:comment "A LocI Dataset is a DCAT and VOID Dataset that has been accepted by the LocI Registry Manager."@en ;
  rdfs:label "LocI Dataset" ;
  rdfs:subClassOf void:Dataset ;
  rdfs:subClassOf dcat:DataService ;
  rdfs:subClassOf [
      a owl:Restriction ;
      owl:minCardinality "1"^^xsd:nonNegativeInteger ;
      owl:onProperty dcat:contactPoint ;
    ] ;
  rdfs:subClassOf [
      a owl:Restriction ;
      owl:onClass org:Organization ;
      owl:onProperty dct:publisher ;
      owl:qualifiedCardinality "1"^^xsd:nonNegativeInteger ;
    ] ;
  rdfs:subClassOf [
      a owl:Restriction ;
      owl:onDataRange xsd:date ;
      owl:onProperty dct:issued ;
      owl:qualifiedCardinality "1"^^xsd:nonNegativeInteger ;
    ] ;
  rdfs:subClassOf [
      a owl:Restriction ;
      owl:onDataRange xsd:date ;
      owl:onProperty dct:modified ;
      owl:qualifiedCardinality "1"^^xsd:nonNegativeInteger ;
    ] ;
  rdfs:subClassOf [
      a owl:Restriction ;
      owl:onDataRange xsd:string ;
      owl:onProperty dct:title ;
      owl:qualifiedCardinality "1"^^xsd:nonNegativeInteger ;
    ] ;
  owl:equivalentClass [
      a owl:Restriction ;
      owl:allValuesFrom :DataPublisher ;
      owl:onProperty dct:publisher ;
    ] ;
.
:DatasetLinkingStatement
  a owl:Class ;
  rdfs:comment "An RDF Statement (Subject, Predicate, Object + additional metadata) that links class instances in one LocI Dataset with class instances in another"@en ;
  rdfs:label "LocI Dataset Linking Statement" ;
  rdfs:subClassOf rdf:Statement ;
  rdfs:subClassOf [
      a owl:Restriction ;
      owl:onClass :Linkset ;
      owl:onProperty reg:register ;
      owl:qualifiedCardinality "1"^^xsd:nonNegativeInteger ;
    ] ;
  rdfs:subClassOf [
      a owl:Restriction ;
      owl:onClass prov:Plan ;
      owl:onProperty :hadGenerationMethod ;
      owl:qualifiedCardinality "1"^^xsd:nonNegativeInteger ;
    ] ;
.
:Feature
  a owl:Class ;
  rdfs:comment "A LocI Feature is just a GeoSPARQL Feature that must have at least one Geometry" ;
  rdfs:label "LocI Feature" ;
  rdfs:subClassOf geo:Feature ;
  rdfs:subClassOf [
      a owl:Restriction ;
      owl:minQualifiedCardinality "1"^^xsd:nonNegativeInteger ;
      owl:onClass geo:Geometry ;
      owl:onProperty geo:hasGeometry ;
    ] ;
.
:Linkset
  a owl:Class ;
  rdfs:comment "A LocI Linkset is a specialised form of a VoID Linkset that requires the void:subjectsTarget & void:objectsTarget indicate LocI Datasets"@en ;
  rdfs:label "LocI Linkset" ;
  rdfs:subClassOf :Dataset ;
  rdfs:subClassOf void:Linkset ;
  owl:equivalentClass [
      a owl:Restriction ;
      owl:allValuesFrom :Dataset ;
      owl:onProperty void:objectsTarget ;
    ] ;
  owl:equivalentClass [
      a owl:Restriction ;
      owl:allValuesFrom :Dataset ;
      owl:onProperty void:subjectsTarget ;
    ] ;
.
:hadGenerationMethod
  a owl:ObjectProperty ;
  rdfs:label "had generation method" ;
  rdfs:range prov:Plan ;
  owl:propertyChainAxiom (
      prov:wasGeneratedBy
      prov:qualifiedAssociation
      prov:hadPlan
    ) ;
  skos:definition "Something (likely a prov:Entity) had a method (prov:Plan) that was used to generate it"@en ;
  skos:editorialNote "This property is a property chain axiome equivalent to a chian of three properties in the PROV ontology: prov:wasGeneratedBy, prov:qualifiedAssociation and prof:hadPlan linking a prov:Entity (the thing generated) to a prov:Plan (the thin instruction generation - the method) via a prov:Activity (the generating event) and a prov:Association that the prov:Activity has linking it to the prov:Plan."@en ;
.
