# baseURI: https://linked.data.gov.au/def/loci
# prefix: loci

@prefix dcat: <http://www.w3.org/ns/dcat#> .
@prefix dcterms: <http://purl.org/dc/terms/> .
@prefix foaf: <http://xmlns.com/foaf/0.1/> .
@prefix geo: <http://www.opengis.net/ont/geosparql#> .
@prefix loci: <https://linked.data.gov.au/def/loci#> .
@prefix owl: <http://www.w3.org/2002/07/owl#> .
@prefix prov: <http://www.w3.org/ns/prov#> .
@prefix rdf: <http://www.w3.org/1999/02/22-rdf-syntax-ns#> .
@prefix rdfs: <http://www.w3.org/2000/01/rdf-schema#> .
@prefix sdo: <https://schema.org/> .
@prefix skos: <http://www.w3.org/2004/02/skos/core#> .
@prefix void: <http://rdfs.org/ns/void#> .
@prefix xsd: <http://www.w3.org/2001/XMLSchema#> .


<https://linked.data.gov.au/def/loci>
  a owl:Ontology ;
  dcterms:created "2018-10-29"^^xsd:date ;
  dcterms:creator <https://orcid.org/0000-0002-3884-3420> ;
  dcterms:creator <https://orcid.org/0000-0002-8742-7730> ;
  dcterms:license <https://creativecommons.org/licenses/by/4.0/> ;
  dcterms:modified "2021-04-01"^^xsd:date ;
  dcterms:publisher <https://linked.data.gov.au/org/csiro> ;  
  dcterms:rights "(c) Commonwealth of Australia (CSIRO), 2021"^^xsd:string ;
  skos:definition """An ontology to describe spatial Linked Data resources as used within the [Loc-I project](https://www.ga.gov.au/locationindex).

This ontology's core taxonomy is Dataset, FeatureCollection, Feature & Geometry which serve to bundle of spatial feature instances and link them to geometries. The secondary taxonomy is Linkset & LinkingStatement whereby links between Datasets are bundled."""@en ;
  skos:prefLabel "Loc-I Ontology"@en ;
  owl:versionIRI <https://linked.data.gov.au/def/loc/2.0> ;
  owl:versionInfo """v2.0:  
* updated to match OGC API requirements;  
* removed unnecissary imports;
* used sdo: in place of org: & doap:"""^^xsd:string ;
  sdo:codeRepository "https://github.com/CSIRO-enviro-informatics/loci-ont"^^xsd:anyURI ;
.
loci:Dataset
  a owl:Class ;
  skos:definition """A Loc-I Dataset is the main management unit of data within the Loc-I project; all Loc-I data must be supplied within Datasets. 
  
  This class is a specialised form (subClassOf) DCAT Dataset & VoID Dataset and is expected to have basic metadata properties, as per DCAT, and may be the target of Linksets linking its elements to other Datasets, as per VoID.
  
  Loc-I Datasets are expected to contain Feature Collections (`loci:FeatureCollection` instances) which in turn contain Features (`loci:Feature` instances) that link to geometry data (`geo:Geometry` instances) and this taxonomy matches the elements of OGC API:Feature APIs."""@en ;
  skos:prefLabel "Dataset"@en ;
  rdfs:subClassOf void:Dataset ;
  rdfs:subClassOf dcat:Dataset ;
  skos:historyNote """Loc-I Ontology versions prior to v2.0 placed restrictions on this class for data validation, however as of v2.0, validation of Loc-I ontology data is expected to be done with contraint language validators (e.g. SHACL), not with ontology rules. Thos validators may target this specialised class for validation. Also, prior to v2.0, this class' definition focussed on governance however this emphasis has been removed in v2.0 and left to non ontology proceeses."""@en ;
.
loci:FeatureCollection
  a owl:Class ;
  rdfs:subClassOf <http://purl.org/dc/dcmitype/Collection> ;
  skos:definition """A Loc-I Feature Collection is a named and described collection of loci:Feature instances.
  
This class is the equivalent to 'collection' in the OGC API:Features specification.

Loc-I Feature Collection instances are always part of one and only one Loc-I Dataset instance and always have an identifier that can be used in OGC API:Feature instance."""@en ;
  skos:prefLabel "Feature Collection"@en ;
  rdfs:subClassOf [
      a owl:Restriction ;
      owl:cardinality "1"^^xsd:nonNegativeInteger ;
      owl:allValuesFrom loci:Dataset ;
      owl:onProperty dcterms:isPartOf ;
  ] ;
  rdfs:subClassOf [
      a owl:Restriction ;
      owl:cardinality "1"^^xsd:nonNegativeInteger ;
      owl:onProperty dcterms:identifier ;
      owl:allValuesFrom xsd:token ;
  ] ;  
.
loci:Feature
  a owl:Class ;
  skos:definition """A Loc-I Feature is a specialised form of GeoSPARQL Feature.

Loc-I Deature instances always have at least one Geometry.

Loc-I Feature instances are always part of one and only one Loc-I FeatureCollection instance and always have an identifier that can be used in OGC API:Feature instance."""@en ;
  skos:prefLabel "Feature"@en ;
  rdfs:subClassOf geo:Feature ;
  rdfs:subClassOf [
      a owl:Restriction ;
      owl:cardinality "1"^^xsd:nonNegativeInteger ;
      owl:allValuesFrom loci:FeatureCollection ;
      owl:onProperty dcterms:isPartOf ;
  ] ;
  rdfs:subClassOf [
      a owl:Restriction ;
      owl:cardinality "1"^^xsd:nonNegativeInteger ;
      owl:onProperty dcterms:identifier ;
      owl:allValuesFrom xsd:token ;
  ] ;
  rdfs:subClassOf [
      a owl:Restriction ;
      owl:cardinality "1"^^xsd:nonNegativeInteger ;
      owl:onProperty geo:hasGeometry ;
      owl:allValuesFrom geo:Geometry ;
  ] ;   
.
loci:LinkingStatement
  a owl:Class ;
  skos:definition """An RDF Statement (Subject, Predicate, Object + additional metadata) that links class instances in one Loc-I Dataset with class instances in another.
  
Linking Statements are always part of a single loci:Linkset instance.

They always indicate the method used to generate them (the Feature/Feature link)."""@en ;
  skos:editorialNote "Linking Statement are just rdf:Statements use as per standard reification practice in VoID for describing links in Linksets however they are distinguished so validation systems can target them separately from any other rdf:Statement instances that may occure elsewhere in Loc-I data."@en ;
  skos:prefLabel "Linking Statement"@en ;
  rdfs:subClassOf rdf:Statement ;
  rdfs:subClassOf [
      a owl:Restriction ;
      owl:cardinality "1"^^xsd:nonNegativeInteger ;
      owl:onProperty rdf:object ;
    ] ;
  rdfs:subClassOf [
      a owl:Restriction ;
      owl:cardinality "1"^^xsd:nonNegativeInteger ;
      owl:onProperty rdf:subject ;
    ] ;
  rdfs:subClassOf [
      a owl:Restriction ;
      owl:minCardinality "1"^^xsd:nonNegativeInteger ;
      owl:onProperty rdf:predicate ;
    ] ;
  rdfs:subClassOf [
      a owl:Restriction ;
      owl:onClass loci:Linkset ;
      owl:onProperty dcterms:isPartOf ;
      owl:qualifiedCardinality "1"^^xsd:nonNegativeInteger ;
    ] ;
  rdfs:subClassOf [
      a owl:Restriction ;
      owl:onClass prov:Plan ;
      owl:onProperty loci:hadGenerationMethod ;
      owl:qualifiedCardinality "1"^^xsd:nonNegativeInteger ;
    ] ;  
.
loci:Linkset
  a owl:Class ;
  skos:definition """A Loc-I Linkset is a specialised form of a VoID Linkset that requires the void:subjectsTarget & void:objectsTarget to indicate Loc-I Datasets.
  
Loc-I Linkset instnaces are expected to contain metadata as per Loc-I Datasets and a list of Loc-I Linking Statements."""@en ;
  skos:prefLabel "Linkset"@en ;
  rdfs:subClassOf loci:Dataset ;
  rdfs:subClassOf void:Linkset ;
  rdfs:subClassOf [
      a owl:Restriction ;
      owl:allValuesFrom loci:LinkingStatement ;
      owl:onProperty rdfs:member ;
    ] ;
  owl:equivalentClass [
      a owl:Restriction ;
      owl:allValuesFrom loci:Dataset ;
      owl:onProperty void:objectsTarget ;
    ] ;
  owl:equivalentClass [
      a owl:Restriction ;
      owl:allValuesFrom loci:Dataset ;
      owl:onProperty void:subjectsTarget ;
    ] ;
.
loci:equivalentTo
  a owl:ObjectProperty ;
  a owl:SymetricProperty ;
  skos:definition """This property is used to relate an individual Feature in one Dataset with a Feature in another Dataset which is intended to represent the same real-world entity.

Use of loci:equivalent would allow representations using slightly different geometrical bases (e.g. surveyed geometries, aggregates of DGGS cells, aggregates of ASGS meshblocks) to be linked, in situations where a purely geometrical computation might not deduce a `geo:sfEquals` relationships because of differing precision, slivers, etc,. When the data provider's intention is that they match, then this predicate can be used to make that assertion. The provenance of the assertion maybe be recorded in the usual way in a Linkset."""@en ;
skos:prefLabel "equivalent to"@en ;
  rdfs:domain geo:Feature ;  
  rdfs:range geo:Feature ;
.
loci:hadGenerationMethod
  a owl:ObjectProperty ;
  rdfs:domain rdf:Statement ;
  skos:prefLabel "had generation method"@en ;
  rdfs:range prov:Plan ;
  owl:propertyChainAxiom (
      prov:wasGeneratedBy
      prov:qualifiedAssociation
      prov:hadPlan
    ) ;
  skos:definition "The method that was used to generate this object"@en ;
  skos:editorialNote "This property is a property chain axiom equivalent to a chain of three properties in the PROV ontology: prov:wasGeneratedBy, prov:qualifiedAssociation and prov:hadPlan linking a prov:Entity (the thing generated) to a prov:Plan (the thin instruction generation - the method) via a prov:Activity (the generating event) and a prov:Association that the prov:Activity has linking it to the prov:Plan."@en ;
.
dcterms:type
  a owl:ObjectProperty ;
  skos:definition """In the context of Loc-I datasets, `dcterms:type` is used for an additional classifier, such as a place-type or meshblock-category. 

The value should be taken from a controlled-vocabulary, and may be expressed as a `skos:Concept` or an `rdfs:Class` or some other kind of resource providing it is from a well-governed source."""@en ;
  skos:prefLabel "type"@en ;
.

<https://linked.data.gov.au/org/csiro>
  a sdo:Organization ;
  sdo:name "CSIRO" ;
  sdo:subjectOf "https://www.csiro.au"^^xsd:anyURI ;
.
<https://orcid.org/0000-0002-3884-3420>
  a sdo:Person ;
  sdo:affiliation <https://linked.data.gov.au/org/csiro> ;
  sdo:identifier "https://orcid.org/0000-0002-3884-3420"^^xsd:anyURI ;
  sdo:name "Simon JD Cox" ;
  sdo:subjectOf <https://people.csiro.au/C/S/simon-cox> ;
.
<https://orcid.org/0000-0002-8742-7730>
  a sdo:Person ;
  sdo:affiliation [
      a sdo:Organization ;
      sdo:name "SURROUND Australia" ;
    ] ;
  sdo:identifier "https://orcid.org/0000-0002-8742-7730"^^xsd:anyURI ;
  sdo:name "Nicholas J. Car" ;
.
