<?xml version="1.0"?>
<rdf:RDF
    xmlns:rdf="http://www.w3.org/1999/02/22-rdf-syntax-ns#"
    xmlns:loci="http://linked.data.gov.au/def/loci#"
    xmlns:sdo="https://schema.org/"
    xmlns:doap="http://usefulinc.com/ns/doap#"
    xmlns:rdfs="http://www.w3.org/2000/01/rdf-schema#"
    xmlns:void="http://rdfs.org/ns/void#"
    xmlns:dcterms="http://purl.org/dc/terms/"
    xmlns:geox="http://linked.data.gov.au/def/geox#"
    xmlns:owl="http://www.w3.org/2002/07/owl#"
    xmlns:prov="http://www.w3.org/ns/prov#"
    xmlns:skos="http://www.w3.org/2004/02/skos/core#"
    xmlns:geo="http://www.opengis.net/ont/geosparql#"
    xmlns:dcat="http://www.w3.org/ns/dcat#"
    xmlns:org="http://www.w3.org/ns/org#"
    xmlns:foaf="http://xmlns.com/foaf/0.1/"
    xmlns:xsd="http://www.w3.org/2001/XMLSchema#"
    xmlns:prof="http://www.w3.org/ns/dx/prof/"
  xml:base="http://linked.data.gov.au/def/loci">
  <prof:Profile rdf:about="">
    <dcterms:creator rdf:datatype="http://www.w3.org/1999/02/22-rdf-syntax-ns#HTML"
    >&lt;a href='https://orcid.org/0000-0002-3884-3420'&gt;Simon J D Cox, CSIRO&lt;/a&gt;</dcterms:creator>
    <owl:imports rdf:resource="http://xmlns.com/foaf/0.1/"/>
    <prof:hasToken rdf:datatype="http://www.w3.org/2001/XMLSchema#token"
    >loci</prof:hasToken>
    <rdfs:comment>An ontology to govern Linked Data resources published within the [Loc-I](https://confluence.csiro.au/display/DIPAAnalyticHubs/Location+Integration+Capability+Loc-I) project.&#xD;
&#xD;
The primary focus is on (a) datasets composed of multiple geospatial features (objects); (b) recording relationships between features, with metadata attached to reified rdf:Statements. </rdfs:comment>
    <dcterms:creator rdf:datatype="http://www.w3.org/1999/02/22-rdf-syntax-ns#HTML"
    >&lt;a href='http://orcid.org/0000-0002-8742-7730'&gt;Nicholas J Car, Surround Australia&lt;/a&gt;</dcterms:creator>
    <dcterms:created rdf:datatype="http://www.w3.org/2001/XMLSchema#date"
    >2018-10-29</dcterms:created>
    <owl:imports rdf:resource="http://vocab.deri.ie/void"/>
    <prof:isProfileOf rdf:resource="http://rdfs.org/ns/void"/>
    <owl:imports rdf:resource="http://www.w3.org/ns/dcat#"/>
    <prof:hasResource>
      <prof:ResourceDescriptor>
        <prof:hasRole rdf:resource="http://www.w3.org/ns/dx/prof/role/specification"/>
        <prof:hasArtifact rdf:resource="http://linked.data.gov.au/def/loci/loci.ttl"/>
        <dcterms:title xml:lang="en">Profile Specification</dcterms:title>
        <dcterms:format rdf:resource="https://w3id.org/mediatype/text/turtle"/>
      </prof:ResourceDescriptor>
    </prof:hasResource>
    <rdf:type rdf:resource="http://www.w3.org/2002/07/owl#Ontology"/>
    <prov:wasGeneratedBy>
      <prov:Activity>
        <rdfs:label>Loc-I project</rdfs:label>
        <doap:repository rdf:resource="https://github.com/CSIRO-enviro-informatics/loci-ont"/>
        <rdf:type rdf:resource="http://usefulinc.com/ns/doap#Project"/>
      </prov:Activity>
    </prov:wasGeneratedBy>
    <owl:versionIRI rdf:resource="http://linked.data.gov.au/def/loci/1.1"/>
    <owl:versionInfo xml:lang="en">Beta version</owl:versionInfo>
    <prof:hasResource>
      <prof:ResourceDescriptor>
        <prof:hasRole rdf:resource="http://www.w3.org/ns/dx/prof/role/constraints"/>
        <prof:hasArtifact rdf:resource="http://linked.data.gov.au/def/loci/constraints.ttl"/>
        <dcterms:title xml:lang="en">Validator Shapes graph</dcterms:title>
        <dcterms:format rdf:resource="https://w3id.org/mediatype/text/turtle"/>
      </prof:ResourceDescriptor>
    </prof:hasResource>
    <owl:imports rdf:resource="http://linked.data.gov.au/def/geox"/>
    <prof:hasResource>
      <prof:ResourceDescriptor>
        <prof:hasRole rdf:resource="http://www.w3.org/ns/dx/prof/role/guidance"/>
        <prof:hasArtifact rdf:resource="http://linked.data.gov.au/def/loci/loci.html"/>
        <dcterms:title xml:lang="en">Guidance document</dcterms:title>
        <dcterms:format rdf:resource="https://w3id.org/mediatype/text/html"/>
      </prof:ResourceDescriptor>
    </prof:hasResource>
    <prof:hasResource>
      <prof:ResourceDescriptor>
        <prof:hasRole rdf:resource="http://www.w3.org/ns/dx/prof/role/guidance"/>
        <prof:hasArtifact rdf:resource="http://linked.data.gov.au/def/loci/images/loci.png"/>
        <dcterms:title xml:lang="en">Ontology overview diagram</dcterms:title>
        <dcterms:format rdf:resource="https://w3id.org/mediatype/image/svg"/>
      </prof:ResourceDescriptor>
    </prof:hasResource>
    <rdfs:label>Loc-I Ontology</rdfs:label>
    <dcterms:modified rdf:datatype="http://www.w3.org/2001/XMLSchema#date"
    >2020-02-04</dcterms:modified>
    <owl:imports rdf:resource="http://www.w3.org/ns/dcat"/>
  </prof:Profile>
  <owl:Class rdf:ID="DataPublisher">
    <rdfs:label>Loc-I Data Publishers</rdfs:label>
    <rdfs:comment xml:lang="en">The set of all approved publishers of Loc-I data, all of whom are known</rdfs:comment>
    <rdfs:subClassOf rdf:resource="http://xmlns.com/foaf/0.1/Group"/>
  </owl:Class>
  <owl:Class rdf:ID="LinkingStatement">
    <rdfs:subClassOf>
      <owl:Restriction>
        <owl:qualifiedCardinality rdf:datatype="http://www.w3.org/2001/XMLSchema#nonNegativeInteger"
        >1</owl:qualifiedCardinality>
        <owl:onProperty>
          <owl:ObjectProperty rdf:ID="hadGenerationMethod"/>
        </owl:onProperty>
        <owl:onClass rdf:resource="http://www.w3.org/ns/prov#Plan"/>
      </owl:Restriction>
    </rdfs:subClassOf>
    <rdfs:subClassOf>
      <owl:Restriction>
        <owl:qualifiedCardinality rdf:datatype="http://www.w3.org/2001/XMLSchema#nonNegativeInteger"
        >1</owl:qualifiedCardinality>
        <owl:onProperty>
          <owl:ObjectProperty rdf:ID="isMemberOf"/>
        </owl:onProperty>
        <owl:onClass>
          <owl:Class rdf:ID="Linkset"/>
        </owl:onClass>
      </owl:Restriction>
    </rdfs:subClassOf>
    <rdfs:label>Loc-I Dataset Linking Statement</rdfs:label>
    <rdfs:comment xml:lang="en">An RDF Statement (Subject, Predicate, Object + additional metadata) that links class instances in one Loc-I Dataset with class instances in another</rdfs:comment>
    <rdfs:subClassOf rdf:resource="http://www.w3.org/1999/02/22-rdf-syntax-ns#Statement"/>
  </owl:Class>
  <owl:Class rdf:ID="Feature">
    <rdfs:subClassOf>
      <owl:Restriction>
        <owl:onProperty rdf:resource="http://www.opengis.net/ont/geosparql#hasGeometry"/>
        <owl:onClass rdf:resource="http://www.opengis.net/ont/geosparql#Geometry"/>
        <owl:minQualifiedCardinality rdf:datatype="http://www.w3.org/2001/XMLSchema#nonNegativeInteger"
        >1</owl:minQualifiedCardinality>
      </owl:Restriction>
    </rdfs:subClassOf>
    <rdfs:label>Loc-I Feature</rdfs:label>
    <rdfs:comment>A Loc-I Feature is a GeoSPARQL Feature that has at least one Geometry</rdfs:comment>
    <rdfs:comment>Might be better implemented as a SHACL shape</rdfs:comment>
    <rdfs:subClassOf rdf:resource="http://www.opengis.net/ont/geosparql#Feature"/>
  </owl:Class>
  <owl:Class rdf:ID="Dataset">
    <rdfs:label>Loc-I Dataset</rdfs:label>
    <rdfs:subClassOf rdf:resource="http://www.w3.org/ns/dcat#Dataset"/>
    <rdfs:subClassOf>
      <owl:Restriction>
        <owl:qualifiedCardinality rdf:datatype="http://www.w3.org/2001/XMLSchema#nonNegativeInteger"
        >1</owl:qualifiedCardinality>
        <owl:onProperty rdf:resource="http://purl.org/dc/terms/title"/>
        <owl:onDataRange rdf:resource="http://www.w3.org/2001/XMLSchema#string"/>
      </owl:Restriction>
    </rdfs:subClassOf>
    <rdfs:subClassOf>
      <owl:Restriction>
        <owl:qualifiedCardinality rdf:datatype="http://www.w3.org/2001/XMLSchema#nonNegativeInteger"
        >1</owl:qualifiedCardinality>
        <owl:onProperty rdf:resource="http://purl.org/dc/terms/modified"/>
        <owl:onDataRange rdf:resource="http://www.w3.org/2001/XMLSchema#date"/>
      </owl:Restriction>
    </rdfs:subClassOf>
    <rdfs:subClassOf>
      <owl:Restriction>
        <owl:qualifiedCardinality rdf:datatype="http://www.w3.org/2001/XMLSchema#nonNegativeInteger"
        >1</owl:qualifiedCardinality>
        <owl:onProperty rdf:resource="http://purl.org/dc/terms/issued"/>
        <owl:onDataRange rdf:resource="http://www.w3.org/2001/XMLSchema#date"/>
      </owl:Restriction>
    </rdfs:subClassOf>
    <rdfs:subClassOf>
      <owl:Restriction>
        <owl:qualifiedCardinality rdf:datatype="http://www.w3.org/2001/XMLSchema#nonNegativeInteger"
        >1</owl:qualifiedCardinality>
        <owl:onProperty rdf:resource="http://purl.org/dc/terms/publisher"/>
        <owl:onClass rdf:resource="http://www.w3.org/ns/org#Organization"/>
      </owl:Restriction>
    </rdfs:subClassOf>
    <rdfs:comment xml:lang="en">A Loc-I Dataset is a DCAT and VOID Dataset that has been accepted by the Loc-I Registry Manager.</rdfs:comment>
    <rdfs:subClassOf>
      <owl:Restriction>
        <owl:onProperty rdf:resource="http://www.w3.org/ns/dcat#contactPoint"/>
        <owl:minCardinality rdf:datatype="http://www.w3.org/2001/XMLSchema#nonNegativeInteger"
        >1</owl:minCardinality>
      </owl:Restriction>
    </rdfs:subClassOf>
    <owl:equivalentClass>
      <owl:Restriction>
        <owl:onProperty rdf:resource="http://purl.org/dc/terms/publisher"/>
        <owl:allValuesFrom rdf:resource="#DataPublisher"/>
      </owl:Restriction>
    </owl:equivalentClass>
    <rdfs:subClassOf rdf:resource="http://rdfs.org/ns/void#Dataset"/>
    <rdfs:subClassOf rdf:resource="http://www.w3.org/1999/02/22-rdf-syntax-ns#Bag"/>
    <rdfs:subClassOf>
      <owl:Restriction>
        <owl:allValuesFrom>
          <owl:Class>
            <owl:unionOf rdf:parseType="Collection">
              <owl:Class rdf:about="#Feature"/>
              <owl:Class rdf:about="#LinkingStatement"/>
            </owl:unionOf>
          </owl:Class>
        </owl:allValuesFrom>
        <owl:onProperty rdf:resource="http://www.w3.org/2000/01/rdf-schema#member"/>
      </owl:Restriction>
    </rdfs:subClassOf>
  </owl:Class>
  <owl:Class rdf:about="#Linkset">
    <owl:equivalentClass>
      <owl:Restriction>
        <owl:onProperty rdf:resource="http://rdfs.org/ns/void#subjectsTarget"/>
        <owl:allValuesFrom rdf:resource="#Dataset"/>
      </owl:Restriction>
    </owl:equivalentClass>
    <owl:equivalentClass>
      <owl:Restriction>
        <owl:onProperty rdf:resource="http://rdfs.org/ns/void#objectsTarget"/>
        <owl:allValuesFrom rdf:resource="#Dataset"/>
      </owl:Restriction>
    </owl:equivalentClass>
    <rdfs:subClassOf>
      <owl:Restriction>
        <owl:onProperty rdf:resource="http://www.w3.org/2000/01/rdf-schema#member"/>
        <owl:allValuesFrom rdf:resource="#LinkingStatement"/>
      </owl:Restriction>
    </rdfs:subClassOf>
    <rdfs:label>Loc-I Linkset</rdfs:label>
    <rdfs:comment xml:lang="en">A Loc-I Linkset is a specialised form of a VoID Linkset that requires the void:subjectsTarget &amp; void:objectsTarget indicate Loc-I Datasets</rdfs:comment>
    <rdfs:subClassOf rdf:resource="http://rdfs.org/ns/void#Linkset"/>
    <rdfs:subClassOf rdf:resource="#Dataset"/>
  </owl:Class>
  <owl:ObjectProperty rdf:about="#isMemberOf">
    <rdfs:subPropertyOf>
      <owl:ObjectProperty>
        <owl:inverseOf rdf:resource="http://www.w3.org/2000/01/rdf-schema#member"/>
      </owl:ObjectProperty>
    </rdfs:subPropertyOf>
    <rdfs:label>is member of</rdfs:label>
    <rdfs:comment>In principle this is just inverse of rdfs:member, but because it is defined in a local namespace, make it a sub-property of the inverse</rdfs:comment>
  </owl:ObjectProperty>
  <owl:ObjectProperty rdf:about="#hadGenerationMethod">
    <skos:definition xml:lang="en">The method that was used to generate this object</skos:definition>
    <owl:propertyChainAxiom rdf:parseType="Collection">
      <rdf:Description rdf:about="http://www.w3.org/ns/prov#wasGeneratedBy"/>
      <rdf:Description rdf:about="http://www.w3.org/ns/prov#qualifiedAssociation"/>
      <rdf:Description rdf:about="http://www.w3.org/ns/prov#hadPlan"/>
    </owl:propertyChainAxiom>
    <skos:editorialNote xml:lang="en">This property is a property chain axiom equivalent to a chain of three properties in the PROV ontology: prov:wasGeneratedBy, prov:qualifiedAssociation and prof:hadPlan linking a prov:Entity (the thing generated) to a prov:Plan (the thin instruction generation - the method) via a prov:Activity (the generating event) and a prov:Association that the prov:Activity has linking it to the prov:Plan.</skos:editorialNote>
    <rdfs:domain rdf:resource="http://www.w3.org/1999/02/22-rdf-syntax-ns#Statement"/>
    <rdfs:range rdf:resource="http://www.w3.org/ns/prov#Plan"/>
    <rdfs:label>had generation method</rdfs:label>
  </owl:ObjectProperty>
</rdf:RDF>

<!-- Created with TopBraid -->
