@prefix : <http://linked.data.gov.au/def/loci#> .
@prefix owl: <http://www.w3.org/2002/07/owl#> .
@prefix rdf: <http://www.w3.org/1999/02/22-rdf-syntax-ns#> .
@prefix xml: <http://www.w3.org/XML/1998/namespace> .
@prefix xsd: <http://www.w3.org/2001/XMLSchema#> .
@prefix rdfs: <http://www.w3.org/2000/01/rdf-schema#> .
@base <http://linked.data.gov.au/def/loci> .

<http://linked.data.gov.au/def/loci> rdf:type owl:Ontology ;
                                      owl:versionIRI <http://linked.data.gov.au/def/loci/1.0> ;
                                      owl:imports <http://purl.org/linked-data/registry> ,


                                                  rdf: ,
                                                  <http://www.w3.org/2002/07/owl> ,
                                                  <http://www.w3.org/ns/dcat> ,
                                                  <http://xmlns.com/foaf/0.1/> ;
                                      <http://purl.org/dc/elements/1.1/creator> "Nicholas J. Car" ;
                                      <http://purl.org/dc/elements/1.1/publisher> "CSIRO" ;
                                      <http://purl.org/dc/terms/created> "2018-10-29"^^xsd:date ;
                                      <http://purl.org/dc/terms/creator> <http://orcid.org/0000-0002-8742-7730> ;
                                      <http://purl.org/dc/terms/modified> "2018-11-09"^^xsd:date ;
                                      <http://purl.org/dc/terms/publisher> <http://catalogue.linked.data.gov.au/org/O-000886> ;
                                      rdfs:comment """A profile of several ontologies implemented to govern Linked Data resources published within the LOC-I project.

This ontology profiles the [GeoSPARQL](http://www.opengeospatial.org/standards/geosparql) and [DCAT v2](https://www.w3.org/TR/vocab-dcat-2/) & [VOID](http://www.w3.org/TR/void/) ontologies and requires that certain properties defined by them be present for several classes of resource that are of particular importance to the [LOC-I project](http://loci.cat).

This ontology constrains both normative instruction on what constitutes LOC-I objects and supplies executable constraints to validate instances. This ontologie's components and its relations to the onologies it profiles are described using the [Profiles Ontology](https://www.w3.org/TR/dx-prof).""" ;
                                      rdfs:label "LOC-I Ontology"@en ;
                                      rdfs:seeAlso "http://github.com/CSIRO-enviro-informatics/loci-ont/"@en ;
                                      owl:versionInfo "Beta version"@en .

#################################################################
#    Annotation properties
#################################################################

###  http://www.w3.org/2002/07/owl#minQualifiedCardinality
owl:minQualifiedCardinality rdf:type owl:AnnotationProperty .


###  http://www.w3.org/2002/07/owl#qualifiedCardinality
owl:qualifiedCardinality rdf:type owl:AnnotationProperty .


###  http://www.w3.org/2004/02/skos/core#member
<http://www.w3.org/2004/02/skos/core#member> rdf:type owl:AnnotationProperty .


#################################################################
#    Object Properties
#################################################################

###  http://linked.data.gov.au/def/loci#hadGenerationMethod
:hadGenerationMethod rdf:type owl:ObjectProperty ;
                     rdfs:comment "The LOCI Dataset Linking Statement had a Method that was used to generate it"@en ;
                     rdfs:label "had generation method" ;
                     rdfs:range <http://www.w3.org/ns/prov#Plan> .


#################################################################
#    Classes
#################################################################

###  http://linked.data.gov.au/def/loci#DataPublisher
:DataPublisher rdf:type owl:Class ;
               owl:equivalentClass [ rdf:type owl:Class ;
                                     owl:oneOf ( <http://catalogue.linked.data.gov.au/org/O-000886>
                                                 <http://catalogue.linked.data.gov.au/org/O-000887>
                                                 <http://catalogue.linked.data.gov.au/org/O-000928>
                                                 <http://catalogue.linked.data.gov.au/org/psma>
                                               )
                                   ] ;
               rdfs:subClassOf <http://xmlns.com/foaf/0.1/Group> .


###  http://linked.data.gov.au/def/loci#Dataset
:Dataset rdf:type owl:Class ;
         owl:equivalentClass [ rdf:type owl:Restriction ;
                               owl:onProperty <http://purl.org/dc/terms/publisher> ;
                               owl:allValuesFrom :DataPublisher
                             ] ;
         rdfs:subClassOf <http://rdfs.org/ns/void#Dataset> ,
                         <http://www.w3.org/ns/dcat#Dataset> ,
                         [ rdf:type owl:Restriction ;
                           owl:onProperty <http://www.w3.org/ns/dcat#contactPoint> ;
                           owl:minCardinality "1"^^xsd:nonNegativeInteger
                         ] ,
                         [ rdf:type owl:Restriction ;
                           owl:onProperty <http://purl.org/dc/terms/publisher> ;
                           owl:qualifiedCardinality "1"^^xsd:nonNegativeInteger ;
                           owl:onClass <http://xmlns.com/foaf/0.1/Organization>
                         ] ,
                         [ rdf:type owl:Restriction ;
                           owl:onProperty <http://purl.org/dc/terms/issued> ;
                           owl:qualifiedCardinality "1"^^xsd:nonNegativeInteger ;
                           owl:onDataRange xsd:date
                         ] ,
                         [ rdf:type owl:Restriction ;
                           owl:onProperty <http://purl.org/dc/terms/modified> ;
                           owl:qualifiedCardinality "1"^^xsd:nonNegativeInteger ;
                           owl:onDataRange xsd:date
                         ] ,
                         [ rdf:type owl:Restriction ;
                           owl:onProperty <http://purl.org/dc/terms/title> ;
                           owl:qualifiedCardinality "1"^^xsd:nonNegativeInteger ;
                           owl:onDataRange xsd:string
                         ] ;
         rdfs:comment "A LOCI Dataset is a DCAT and VOID Dataset that has been accepted by the LOCI Registry Manager."@en ;
         rdfs:label "LOCI Dataset" .


###  http://linked.data.gov.au/def/loci#DatasetLinkingStatement
:DatasetLinkingStatement rdf:type owl:Class ;
                         rdfs:subClassOf rdf:Statement ,
                                         [ rdf:type owl:Restriction ;
                                           owl:onProperty :hadGenerationMethod ;
                                           owl:qualifiedCardinality "1"^^xsd:nonNegativeInteger ;
                                           owl:onClass <http://www.w3.org/ns/prov#Plan>
                                         ] ,
                                         [ rdf:type owl:Restriction ;
                                           owl:onProperty <http://purl.org/linked-data/registry#register> ;
                                           owl:qualifiedCardinality "1"^^xsd:nonNegativeInteger ;
                                           owl:onClass :Linkset
                                         ] ,
                                         [ rdf:type owl:Restriction ;
                                           owl:onProperty rdf:object ;
                                           owl:qualifiedCardinality "1"^^xsd:nonNegativeInteger ;
                                           owl:onClass :Feature
                                         ] ,
                                         [ rdf:type owl:Restriction ;
                                           owl:onProperty rdf:subject ;
                                           owl:qualifiedCardinality "1"^^xsd:nonNegativeInteger ;
                                           owl:onClass :Feature
                                         ] ;
                         rdfs:comment "An RDF Statement (Subject, Predicate, Object + additional metadata) that links class instances in one LOCI Dataset with class instances in another"@en ;
                         rdfs:label "LOCI Dataset Linking Statement" .


###  http://linked.data.gov.au/def/loci#Feature
:Feature rdf:type owl:Class ;
         rdfs:subClassOf <http://www.opengis.net/ont/geosparql#Feature> ;
         rdfs:label "LOCI Feature" .


###  http://linked.data.gov.au/def/loci#Linkset
:Linkset rdf:type owl:Class ;
         owl:equivalentClass [ rdf:type owl:Restriction ;
                               owl:onProperty <http://rdfs.org/ns/void#objectsTarget> ;
                               owl:allValuesFrom :Dataset
                             ] ,
                             [ rdf:type owl:Restriction ;
                               owl:onProperty <http://rdfs.org/ns/void#subjectsTarget> ;
                               owl:allValuesFrom :Dataset
                             ] ;
         rdfs:subClassOf :Dataset ,
                         <http://rdfs.org/ns/void#Linkset> ;
         rdfs:comment "A LOCI Linkset is a specialised form of a VOID Linkset that requires the void:subjectsTarget & void:objectsTarget indicate LOCI Datasets"@en ;
         rdfs:label "LOCI Linkset" .


###  http://www.w3.org/1999/02/22-rdf-syntax-ns#Statement
rdf:Statement rdf:type owl:Class .


#################################################################
#    Individuals
#################################################################

###  http://catalogue.linked.data.gov.au/org/O-000886
<http://catalogue.linked.data.gov.au/org/O-000886> rdf:type owl:NamedIndividual ,
                                                            <http://xmlns.com/foaf/0.1/Organization> ;
                                                   rdfs:label "CSIRO" .


###  http://catalogue.linked.data.gov.au/org/O-000887
<http://catalogue.linked.data.gov.au/org/O-000887> rdf:type owl:NamedIndividual ,
                                                            <http://xmlns.com/foaf/0.1/Organization> ;
                                                   rdfs:label "Geoscience Australia" .


###  http://catalogue.linked.data.gov.au/org/O-000928
<http://catalogue.linked.data.gov.au/org/O-000928> rdf:type owl:NamedIndividual ,
                                                            <http://xmlns.com/foaf/0.1/Organization> ;
                                                   rdfs:label "Australian Bureau of Statistics" .


###  http://catalogue.linked.data.gov.au/org/psma
<http://catalogue.linked.data.gov.au/org/psma> rdf:type owl:NamedIndividual ,
                                                        <http://xmlns.com/foaf/0.1/Organization> ;
                                               rdfs:label "PSMA Australia" .


###  http://linked.data.gov.au/dataset/asgs
<http://linked.data.gov.au/dataset/asgs> rdf:type owl:NamedIndividual ,
                                                  :Dataset ;
                                                  rdfs:label "ASGS Dataset" .


###  http://linked.data.gov.au/dataset/geofabric
<http://linked.data.gov.au/dataset/geofabric> rdf:type owl:NamedIndividual ,
                                                       :Dataset ;
                                                       rdfs:label "Geofabric Dataset" .


###  http://linked.data.gov.au/dataset/gnaf
<http://linked.data.gov.au/dataset/gnaf> rdf:type owl:NamedIndividual ,
                                                  :Dataset ;
                                                  rdfs:label "GNAF Dataset" .


###  http://linked.data.gov.au/def/loci#AddressesCatchments
:AddressesCatchments rdf:type owl:NamedIndividual ,
                              :Linkset ;
                              rdfs:label "Addresses Catchments Linkset" .


###  http://linked.data.gov.au/def/loci#DataPublisher
:DataPublisher rdf:type owl:NamedIndividual .


[ owl:qualifiedCardinality "1"^^xsd:nonNegativeInteger
] .

[ owl:qualifiedCardinality "1"^^xsd:nonNegativeInteger
 ] .

[ owl:qualifiedCardinality "1"^^xsd:nonNegativeInteger
 ] .

[ owl:qualifiedCardinality "1"^^xsd:nonNegativeInteger
 ] .

[ owl:minQualifiedCardinality "1"^^xsd:nonNegativeInteger
 ] .

[ owl:qualifiedCardinality "1"^^xsd:nonNegativeInteger
 ] .

#################################################################
#    Annotations
#################################################################

:DataPublisher rdfs:label "LOCI Data Publishers" ;
                rdfs:comment "The set of all approved publishers of LOCI data, all of whom are known"@en .


###  Generated by the OWL API (version 4.5.6.2018-09-06T00:27:41Z) https://github.com/owlcs/owlapi
